fixing state transformers
composition was applied in the wrong direction + not all side effects were zeroed-out

Cook_Levin/IMP-_To_SAS+/IMP-_To_IMP--/Binary_Arithmetic_IMP.thy
@@ -71,17 +71,18 @@ definition nth_bit_of_num_iteration::pcom  where "nth_bit_of_num_iteration \<equ
   [''tl''] ''xs'' ::=  (A ( V ''x'')) ;;
    invoke_subprogram ''tl'' tl_IMP;;
    ''x'' ::= [''tl''] (A (V ''ans''));;
+   [''tl''] ''ans'' ::= A (N 0);;
    ''n'' ::= (V ''n'' \<ominus> N 1 );; 
     nth_bit_of_num_if
 "
 
 definition nth_bit_of_num_iteration_t :: "nat \<Rightarrow> nat \<Rightarrow> nat" where 
-"nth_bit_of_num_iteration_t x n = 6 + tl_time x + nth_bit_of_num_if_time (tl_nat x) (n-1)"
+"nth_bit_of_num_iteration_t x n = 8 + tl_time x + nth_bit_of_num_if_time (tl_nat x) (n-1)"
 
 abbreviation nth_bit_of_num_iteration_state_transformer 
   where "nth_bit_of_num_iteration_state_transformer p x n \<equiv>
-    state_transformer p [(''x'', tl_nat x),(''n'',n-1)] o tl_state_transformer (''tl'' @ p) x
-  o nth_bit_of_num_if_state_transformer p (tl_nat x) (n-1)
+     nth_bit_of_num_if_state_transformer p (tl_nat x) (n-1) o  state_transformer (''tl'' @ p) [( ''ans'', 0)] o
+ tl_state_transformer (''tl'' @ p) x o  state_transformer p [(''x'', tl_nat x),(''n'',n-1)] 
 "
 value "nth_bit_of_num_iteration_state_transformer"
 lemma nth_bit_of_num_iteration_correct[intro]:
@@ -91,7 +92,23 @@ nth_bit_of_num_iteration_state_transformer p x n s"
   unfolding nth_bit_of_num_iteration_def nth_bit_of_num_iteration_t_def
   apply (rule terminates_in_time_state_intro)
     apply (rule Big_StepT.Seq)+
-  by fastforce+
+              apply fastforce
+ apply fastforce
+ apply fastforce
+ apply fastforce
+ apply fastforce
+ apply fastforce
+ apply fastforce
+ apply fastforce
+ apply fastforce
+ apply fastforce
+ apply fastforce
+   apply fastforce
+by fastforce
+  
+  
+
+
 
 
 definition nth_bit_of_num_loop :: "pcom" where 
@@ -110,16 +127,22 @@ fun nth_bit_of_num_loop_state_transformer ::
 "nth_bit_of_num_loop_state_transformer p 0 x n = id "|
 "nth_bit_of_num_loop_state_transformer p (Suc b) x n = (let x' = tl_nat x; n' = n-1;
 iteration = nth_bit_of_num_iteration_state_transformer p x n  in 
-(if x'>0 \<and> n'>0 then iteration o nth_bit_of_num_loop_state_transformer p (Suc 0) x' n' else
-iteration
-o nth_bit_of_num_loop_state_transformer p 0 x' n'
+(if x'>0 \<and> n'>0 then nth_bit_of_num_loop_state_transformer p (Suc 0) x' n' o iteration else
+nth_bit_of_num_loop_state_transformer p 0 x' n' o iteration
  ))"
 
-lemma " (nth_bit_of_num_iteration_state_transformer p x n
-         o nth_bit_of_num_loop_state_transformer p (Suc 0) (tl_nat x) (n-1)) s = 
-      (nth_bit_of_num_loop_state_transformer p (Suc 0) (tl_nat x) (n-1)) s"
-  apply (induction p "Suc 0" "tl_nat x" "n-1" arbitrary: x n s rule:nth_bit_of_num_loop_state_transformer.induct)
+lemma "
+(nth_bit_of_num_iteration_state_transformer p (tl_nat x) (n-1) o
+     nth_bit_of_num_iteration_state_transformer p x n) s = nth_bit_of_num_iteration_state_transformer p (tl_nat x) (n-1) s 
+"
+  sledgehammer
+lemma " x' = tl_nat x \<Longrightarrow> n' = n-1 \<Longrightarrow> x>0 \<Longrightarrow> n> 0 \<Longrightarrow>
+             (nth_bit_of_num_loop_state_transformer p (Suc 0) x' n'
+o nth_bit_of_num_iteration_state_transformer p x n ) s = 
+      (nth_bit_of_num_loop_state_transformer p (Suc 0) x' n') s"
+  apply (induction  x' n' arbitrary: x n s rule:nth_bit_of_num_nat.induct)
   apply auto
+  apply fastforce
 fun nth_bit_of_num_loop_state_transformer' ::
 "char list \<Rightarrow> nat \<Rightarrow> nat \<Rightarrow> nat \<Rightarrow> (char list \<Rightarrow> nat) \<Rightarrow> char list \<Rightarrow> nat" where 
 "nth_bit_of_num_loop_state_transformer' p 0 x n = id "|
@@ -167,14 +190,15 @@ case (1)
    using 1  by auto
 next
   case (2 v)
-  obtain s' where s'_def: "s' =state_transformer p
-      [(''x'', tl_nat (s (add_prefix p ''x''))), (''n'', s (add_prefix p ''n'') - Suc 0)]
-      (state_transformer (CHR ''t'' # CHR ''l'' # p)
-        [(''ans'', tl_nat (s (add_prefix p ''x''))), (''xs'', 0)]
-        (snd_nat_IMP_Minus_state_transformer
-          (CHR ''s'' # CHR ''n'' # CHR ''d'' # CHR ''t'' # CHR ''l'' # p)
-          (s (add_prefix p ''x'') - Suc 0)
-          (state_transformer p [(''b'', Suc 0)] s)))" by simp
+  obtain s' where s'_def: "s' = (state_transformer p
+       [(''b'',
+         if 0 < tl_nat (s (add_prefix p ''x'')) \<and> 0 < s (add_prefix p ''n'') - 1 then 1
+         else 0)] \<circ>
+      state_transformer (''tl'' @ p) [(''ans'', 0)] \<circ>
+      tl_state_transformer (''tl'' @ p) (s (add_prefix p ''x'')) \<circ>
+      state_transformer p
+       [(''x'', tl_nat (s (add_prefix p ''x''))), (''n'', s (add_prefix p ''n'') - 1)])
+      s" by simp
     show ?case 
       apply(rule terminates_in_time_state_intro [where s'= "if  0 < tl_nat (s (add_prefix p ''x'')) \<and> 0 < s (add_prefix p ''n'') - 1 then s1 else s2"  
      for s1 s2] )
@@ -186,18 +210,13 @@ next
             apply simp
            apply simp
        apply(rule terminates_split_if)
-       using 2(1)[of s'] s'_def  apply force
-       using 2(2)[of s'] s'_def apply force
+       using 2(1)[of s'] s'_def apply fastforce
+       using 2(2)[of s'] s'_def apply fastforce
          apply fastforce
        using 2(3)[symmetric] apply auto[1]
        apply (smt (z3) One_nat_def less_diff_conv plus_1_eq_Suc) 
-       using 2(3)[symmetric] apply (simp only:)
-       apply (subst (2) nth_bit_of_num_loop_state_transformer.simps)
-        
-       apply (afuto simp add: Let_def simp del: nth_bit_of_num_loop_state_transformer.simps(2))
-       slefdgehammer
-         apply (auto simp only:Let_def One_nat_def  comp_apply One_nat_def less_diff_conv plus_1_eq_Suc)
-       apply (auto simp)    
+       using 2(3)[symmetric] apply auto
+       apply (auto simp only:Let_def comp_apply)
        
 qed
 
