IMP-/Big_StepT.thy
@@ -72,7 +72,6 @@ inductive_cases Assign_tE[elim!]: "(x ::= a,s) \<Rightarrow>\<^bsup> p \<^esup> 
 inductive_cases Seq_tE[elim!]: "(c1;;c2,s1) \<Rightarrow>\<^bsup> p \<^esup> s3"
 inductive_cases If_tE[elim!]: "(IF b \<noteq>0 THEN c1 ELSE c2,s) \<Rightarrow>\<^bsup> x \<^esup> t"
 inductive_cases While_tE[elim]: "(WHILE b \<noteq>0 DO c,s) \<Rightarrow>\<^bsup> x \<^esup> t"
-
 lemma Seq': "\<lbrakk> (c1,s1) \<Rightarrow>\<^bsup> x \<^esup> s2;  (c2,s2) \<Rightarrow>\<^bsup> y \<^esup> s3  \<rbrakk> \<Longrightarrow> (c1;;c2, s1) \<Rightarrow>\<^bsup> x + y \<^esup> s3"
   by auto
 
@@ -204,5 +203,9 @@ lemma terminates_in_state_intro: "(c, s) \<Rightarrow>\<^bsup>t\<^esup> s' \<Lon
 lemma terminates_in_time_state_intro: "(c, s) \<Rightarrow>\<^bsup>t\<^esup> s' \<Longrightarrow> t = t' \<Longrightarrow> s' = s'' 
   \<Longrightarrow> (c, s) \<Rightarrow>\<^bsup>t'\<^esup> s''"
   by simp
+
+lemma terminates_split_if : "(P s \<Longrightarrow> (c, s) \<Rightarrow>\<^bsup>t1\<^esup> s1 ) \<Longrightarrow> 
+(\<not> P s \<Longrightarrow> (c, s) \<Rightarrow>\<^bsup>t2\<^esup> s2 ) \<Longrightarrow> (c,s) \<Rightarrow>\<^bsup>if P s then t1 else t2\<^esup>  if P s then s1 else s2"
+  by auto
 
 end
